examples/layeredeffects/AlgForAll.fst
@@ -1,0 +1,178 @@
+module AlgForAll
+
+open Common
+open FStar.Calc
+module WF = FStar.WellFounded
+module FE = FStar.FunctionalExtensionality
+module F = FStar.FunctionalExtensionality
+module W = FStar.WellFounded
+module T = FStar.Tactics
+open LatticeAlg
+
+
+let pre = state -> Type0
+let post (a:Type) = a -> state -> Type0
+let st_wp (a:Type) : Type = post a -> pre
+
+let return_wp #a x : st_wp a = fun p s -> p x s 
+
+let bind_wp #a #b (w : st_wp a) (wf : a -> st_wp b)
+  : st_wp b
+  = fun p s0 -> w (fun y s1 -> wf y p s1) s0
+
+let read_wp : st_wp state = fun p s0 -> p s0 s0
+
+let write_wp : state -> st_wp unit = fun s p _ -> p () s
+
+(* Also doable with handlers *)
+let rec interp_as_wp #a (t : repr a [Read;Write]) : st_wp a =
+  match t with
+  | Return x -> return_wp x
+  | Act Read _ k ->
+    bind_wp read_wp (fun s -> WF.axiom1 k s; interp_as_wp (k s))
+  | Act Write s k ->
+    bind_wp (write_wp s) (fun () -> WF.axiom1 k (); interp_as_wp (k ()))
+  
+// m is a monad.
+val m (a : Type u#a) : Type u#a
+let m a = repr a [Read;Write]
+
+val m_return (#a : Type) : a -> m a
+let m_return x = Return x
+
+val m_bind (#a #b : Type) : m a -> (a -> m b) -> m b
+let m_bind c f = bind _ _ _ _ c f
+
+val w (a : Type u#a) : Type u#(max 1 a)
+let w = st_wp
+
+val w_return (#a : Type) : a -> w a
+let w_return = return_wp
+
+val w_bind (#a #b : Type) : w a -> (a -> w b) -> w b
+let w_bind = bind_wp
+
+val stronger : (#a:Type) -> FStar.Preorder.preorder (w a)
+let stronger w1 w2 = forall p s. w1 p s ==> w2 p s
+
+let equiv #a (w1 w2 : w a) = w1 `stronger` w2 /\ w2 `stronger` w1
+
+let bind_is_monotonic
+  (#a #b : Type)
+  (w1 w2 : w a) 
+  (f1 f2 : a -> w b)
+  : Lemma (requires (w1 `stronger` w2 /\ (forall x. f1 x `stronger` f2 x)))
+          (ensures (w_bind w1 f1 `stronger` w_bind w2 f2))
+  = admit ()
+
+let (<<=) = stronger
+
+// a morphism between them, satisfying appropriate laws
+val interp (#a : Type) : m a -> w a
+let interp = interp_as_wp
+
+val interp_ret (#a:Type) (x:a)
+  : Lemma (interp (m_return x) `equiv` w_return x)
+let interp_ret x = assert (interp (m_return x) `equiv` w_return x) by (T.compute ())
+
+val interp_bind (#a #b:Type)
+  (c : m a) (f : a -> m b)
+  : Lemma (interp (m_bind c f) `equiv` w_bind (interp c) (fun x -> interp (f x)))
+let interp_bind c f =
+  calc equiv {
+    interp (m_bind c f);
+    equiv { admit() }
+    w_bind (interp c) (fun x -> interp (f x));
+  }
+
+let repr (a : Type) (w: w a) = c:(m a){w `stronger` interp c}
+
+let return (a:Type) (x:a) : repr a (w_return x) =
+  interp_ret x;
+  m_return x
+
+let bind (a : Type) (b : Type)
+  (wp_v : w a) (wp_f: a -> w b)
+  (v : repr a wp_v) (f : (x:a -> repr b (wp_f x)))
+  : repr b (w_bind wp_v wp_f) =
+  let r = m_bind v f in
+  (* Proof that stronger holds *)
+  calc (<<=) {
+    w_bind wp_v wp_f;
+    <<= { bind_is_monotonic wp_v (interp v) wp_f (fun x -> interp (f x)) (* from the refinement *) }
+    w_bind (interp v) (fun x -> interp (f x));
+    <<= { interp_bind v f }
+    interp (m_bind v f);
+  };
+  r
+  
+let subcomp (a:Type) (w1 w2: w a)
+  (f : repr a w1)
+  : Pure (repr a w2)
+         (requires w2 `stronger` w1)
+         (ensures fun _ -> True)
+  = f
+
+let if_then_else (a : Type) (w1 w2 : w a) (f : repr a w1) (g : repr a w2) (b : bool) : Type =
+  repr a (if b then w1 else w2)
+
+total
+reifiable
+reflectable
+layered_effect {
+  DM4A : a:Type -> w a -> Effect
+  with repr         = repr;
+       return       = return;
+       bind         = bind;
+       subcomp      = subcomp; 
+       if_then_else = if_then_else
+}
+
+let _get : repr state read_wp =
+  let c0 : LatticeAlg.repr state [Read;Write] = LatticeAlg._get in
+  let w = interp_as_wp c0 in
+  assert_norm (read_wp `stronger` w);
+  c0
+
+let get () : DM4A state read_wp =
+  DM4A?.reflect _get
+  
+let _put (s:state) : repr unit (write_wp s) =
+  let c0 : LatticeAlg.repr unit [Read;Write] = LatticeAlg._put s in
+  let w = interp_as_wp c0 in
+  assert_norm (write_wp s `stronger` w);
+  c0
+
+let put (s:state) : DM4A unit (write_wp s) =
+  DM4A?.reflect (_put s)
+
+let lift_pure_wp (#a:Type) (wp : pure_wp a) : st_wp a =
+  fun p s0 -> wp (fun x -> p x s0)
+ 
+let lift_pure_dm4a (a:Type) wp (f:(eqtype_as_type unit -> PURE a wp))
+  : Pure (repr a (lift_pure_wp wp)) // can't call f() here, so lift its wp instead
+         (requires (wp (fun _ -> True)))
+         (ensures (fun _ -> True))
+  = 
+    let v : a = elim_pure f (fun _ -> True) in
+    FStar.Monotonic.Pure.wp_monotonic_pure ();
+    assert (forall p. wp p ==> p v); // this is key fact needed for the proof
+    assert_norm (stronger (lift_pure_wp wp) (w_return v));
+    Return v
+
+sub_effect PURE ~> DM4A = lift_pure_dm4a
+
+[@@expect_failure] // lift doesn't really work
+let test () : DM4A int (w_return 5) = r 5
+
+let addx (x:int) : DM4A unit (fun p s0 -> p () (s0+x)) by (T.norm [delta]) =
+  let y = get () in
+  put (x+y)
+
+let add_via_state (x y : int) : DM4A int (fun p s0 -> p (x+y) s0) by (T.norm [delta]) =
+  let o = get () in
+  put x;
+  addx y;
+  let r = get () in
+  put o;
+  r
